\documentclass[journal, 12pt, twocolumn]{IEEEtran}
\usepackage[utf8]{inputenc}
\usepackage{graphicx}
\usepackage{amssymb}
\usepackage{amsmath}
\graphicspath{{figs/}}
\title{AI1110 Assignment 1}
\author{Donal Loitam(AI21BTECH11009)}

\begin{document}
    \maketitle

    \textbf{\large{ICSE class 10 paper 2019}}\\
    \\
    \\
    {Q2 (C):
    In an Arithmetic Progression, the fourth and sixth terms are 8 and 16 respectively.Find :\\
 i) common difference\\
 ii) first term\\
 iii) sum of the first 20 terms}\\\\\\
    \textbf{\large{Solution:}}
    Let $a_i$\text { denote the i th term of the AP }, 
 \(d\)\text{ denote the common diff,} 
$S_{20}$\text{ denote the sum of first 20 terms}\\

\begin{table}[h!]
\caption{Variables}
    \centering
    \begin{tabular}{|c|c|}
        \hline
        Symbol & value \\
        $ i $  &  4   \\
         $ j $  &  6   \\
         $ a_i $ &  8  \\
         $ a_j $ & 14  \\
         $ a_1 $ &  ?  \\
            d    &  ?  \\
        $S_{n}$  &  ?  \\
       $S_{20}$  &  ?  \\
          \hline
    \end{tabular}
\end{table}
    


\textbf{For any general $a_i$ , $a_j$ :}\\
\begin{align*}
        &(i)&a_i + (j-i)d &= a_j\\
        &\Rightarrow & (j-i)d &= a_j - a_i\\
        &\Rightarrow & (j-i)d &= 14 - 8\\
        &\Rightarrow & (j-i)d &= 6\\
        &\Rightarrow & d  &= \tfrac{6}{(j-i)} \tag{1}\\ 
    \end{align*}
Substituting  $i=4$ and $j=6$ in eq.(1):
\begin{align*}
    & \Rightarrow & d  &= \tfrac{6}{6-4} \\
    & \Rightarrow & d  &= \tfrac{6}{2} \\
        &  \therefore  & d  &=  3 \tag{2}  \\
\end{align*}
    
    
     \begin{align*}
        &(ii)&a_1 + (i-1)d &= a_i\\
        &\Rightarrow & a_1 &= a_i - (i-1)d\\
        &\Rightarrow & a_1 &=  a_i - \tfrac{(i-1)6}{(j-i)} \;\;\;\\ 
        &\Rightarrow & a_1 &=  \tfrac{a_i(j-i)\;-\;6(i-1)}{(j-i)} \tag{3}\;\\
         \end{align*}
Substituting $i=4,j=6$ and $a_i=8$ in eq.(3):
\begin{align*}
    &\Rightarrow & a_1 &=  \tfrac{8(6-4)\;-\;6(4-1)}{(6-4)} \;\\
         &\Rightarrow & a_1 &=  \tfrac{8(2)\;-\;6(3)}{(2)} \;\\
         &\Rightarrow & a_1 &=  \tfrac{16\;-\;18}{2} \\ 
          &\therefore &  a_1 &=\tfrac{-2}{2} = -1 \tag{4}\\
\end{align*}         
    
Now calculating $S_n$ for general n:   
    \begin{align*}
        iii)  S_{n} &= a_1 + a_2 + ......... + a_{20}\\
               &= \tfrac{n\;\times\;\left[2a_1 + (n-1)d\right]}{2} \tag{5}\\
    \end{align*} 
Using values from eq.(2) and eq.(4) in eq.(5):
\begin{align*}
    &  & S_{n}  &= \tfrac{n\;\times\;\left[2(-1) + (n-1)3\right]}{2}\\
   &  \therefore  & S_n  &=  \tfrac{n\;\times\;\left[3(n-1) - 2\right]}{2}\tag{6}\\
\end{align*}

Substituting $n=20$ in eq.(6) 
 \begin{align*}
    &  & S_{20}  &= \tfrac{20\;\times\;\left[3(20-1) - 2\right]}{2}\\
   &  \Rightarrow  & S_{20}  &=  10\times[3(19)-2]\\
   &  \Rightarrow  & S_{20}  &=  10\times[57-2]\\
   &  \therefore  & S_{20}  &=  10\times[55] = 550
\end{align*}

    
    
\end{document}